.

GIT_nova.v
@@ -178,785 +178,124 @@ End Preliminaries.
 
 Section Arithmetic.
 
-Definition arity : Set :=
-  nat
-.
-
-Inductive Arith : Set :=
-| varArith : arity -> Arith
-| plusArith : Arith -> Arith -> Arith
-| multArith : Arith -> Arith -> Arith
-| ltArith : Arith -> Arith -> Arith
-| muArith : Arith -> Arith
-.
-
 Definition w : Set :=
   nat
 .
 
-Fixpoint Lift (ary : arity) (A : Type) : Type :=
-  match ary with
+Fixpoint Arity (n : nat) (A : Type) : Type :=
+  match n with
   | 0 => A
-  | S ary' => w -> Lift ary' A
+  | S n' => w -> Arity n' A
   end
 .
 
-Fixpoint unLiftProp (ary : arity) : Lift ary Prop -> Prop :=
-  match ary with
+Fixpoint universal (n : nat) : Arity n Prop -> Prop :=
+  match n with
   | 0 =>
     fun P : Prop =>
     P
-  | S ary' =>
-    fun A : w -> Lift ary' Prop =>
-    forall n : w, unLiftProp ary' (A n)
-  end
-.
-
-Fixpoint returnLift {A : Type} (ary : arity) : A -> Lift ary A :=
-  match ary with
-  | 0 =>
-    fun x : A =>
-    x
-  | S ary' =>
-    fun x : A =>
-    fun _ : w =>
-    returnLift ary' x
-  end
-.
-
-Fixpoint bindLift {A : Type} {B : Type} (ary : arity) : Lift ary A -> (A -> Lift ary B) -> Lift ary B :=
-  match ary with
-  | 0 =>
-    fun x : A =>
-    fun f : A -> B =>
-    f x
-  | S ary' =>
-    fun x : w -> Lift ary' A =>
-    fun f : A -> w -> Lift ary' B =>
-    fun w : nat =>
-    bindLift ary' (x w) (fun a : A => f a w)
-  end
-.
-
-Fixpoint shiftLift_left {A : Type} (ary : arity) : Lift (S ary) A -> Lift ary (w -> A) :=
-  match ary with
-  | 0 =>
-    fun f : w -> A =>
-    f
-  | S ary' =>
-    fun f : w -> Lift (S ary') A =>
-    fun x : w =>
-    shiftLift_left ary' (f x)
-  end
-.
-
-Fixpoint shiftLift_right {A : Type} (ary : arity) : Lift ary (w -> A) -> Lift (S ary) A :=
-  match ary with
-  | 0 =>
-    fun f : w -> A =>
-    f
-  | S ary' =>
-    fun f : w -> Lift ary' (w -> A) =>
-    fun x : w =>
-    shiftLift_right ary' (f x)
-  end
-.
-
-Definition apLift {A : Type} {B : Type} (ary : arity) (f : Lift ary (A -> B)) (x : Lift ary A) : Lift ary B :=
-  bindLift ary f (fun f' : A -> B => bindLift ary x (fun x' : A => returnLift ary (f' x')))
-.
-
-Fixpoint assocLift {A : Type} (n : arity) : forall ary, Lift n (Lift ary A) -> Lift (n + ary) A :=
-  match n with
-  | 0 =>
-    fun ary : arity =>
-    fun f : Lift ary A =>
-    f
   | S n' =>
-    fun ary : arity =>
-    fun f : w -> Lift n' (Lift ary A) =>
-    fun x : w =>
-    assocLift n' ary (f x)
+    fun P : w -> Arity n' Prop =>
+    forall m : nat, universal n' (P m)
   end
 .
 
-Lemma assoc_return :
-  forall ary : arity,
-  returnLift (ary + 0) 0 = assocLift ary 0 (returnLift ary 0).
-Proof with eauto.
-  induction ary... simpl. rewrite IHary...
-Qed.
-
-Definition projection (n : arity) (m : arity) : Lift (m + S n) w :=
-  assocLift m (S n) (returnLift m (returnLift n))
+Fixpoint pureArity {A : Type} (n : nat) : A -> Arity n A :=
+  match n with
+  | 0 => fun x : A => x
+  | S n' => fun x : A => fun m : w => pureArity n' x
+  end
 .
 
-Example projection_ex1 : projection 0 4 = (fun x4 : w => fun x3 : w => fun x2 : w => fun x1 : w => fun x0 : w => x0) := eq_refl.
-
-Example projection_ex2 : projection 1 3 = (fun x4 : w => fun x3 : w => fun x2 : w => fun x1 : w => fun x0 : w => x1) := eq_refl.
-
-Example projection_ex3 : projection 2 2 = (fun x4 : w => fun x3 : w => fun x2 : w => fun x1 : w => fun x0 : w => x2) := eq_refl.
-
-Example projection_ex4 : projection 3 1 = (fun x4 : w => fun x3 : w => fun x2 : w => fun x1 : w => fun x0 : w => x3) := eq_refl.
-
-Example projection_ex5 : projection 4 0 = (fun x4 : w => fun x3 : w => fun x2 : w => fun x1 : w => fun x0 : w => x4) := eq_refl.
-
-Definition chi_lt (x : w) (y : w) : w :=
-  if Compare_dec.lt_dec x y then 0 else 1
+Fixpoint apArity {A : Type} {B : Type} (n : nat) : Arity n (A -> B) -> Arity n A -> Arity n B :=
+  match n with
+  | 0 => fun f : A -> B => fun x : A => f x
+  | S n' => fun f : w -> Arity n' (A -> B) => fun x : w -> Arity n' A => fun m : w => apArity n' (f m) (x m)
+  end
 .
 
-Definition check (ary : arity) (val : Lift (S ary) w) : Lift ary (w -> bool) :=
-  apLift ary (returnLift ary (fun f : w -> w => fun x : w => Nat.eqb (f x) 0)) (shiftLift_left ary val)
+Definition liftArity1 {A : Type} {B : Type} (n : nat) : (A -> B) -> Arity n A -> Arity n B :=
+  fun f : A -> B => fun val1 : Arity n A => apArity n (pureArity n f) val1
 .
 
-Inductive evalArith : forall ary : arity, Arith -> Lift ary w -> Prop :=
-| varEval :
-  forall m : arity,
-  forall n : arity,
-  evalArith (m + S n) (varArith n) (projection n m)
-| plusEval :
-  forall ary : arity,
-  forall val1 : Lift ary w,
-  forall val2 : Lift ary w,
-  forall e1 : Arith,
-  forall e2 : Arith,
-  evalArith ary e1 val1 ->
-  evalArith ary e2 val2 ->
-  evalArith ary (plusArith e1 e2) (apLift ary (apLift ary (returnLift ary plus) val1) val2)
-| multEval :
-  forall ary : arity,
-  forall val1 : Lift ary w,
-  forall val2 : Lift ary w,
-  forall e1 : Arith,
-  forall e2 : Arith,
-  evalArith ary e1 val1 ->
-  evalArith ary e2 val2 ->
-  evalArith ary (multArith e1 e2) (apLift ary (apLift ary (returnLift ary mult) val1) val2)
-| ltEval :
-  forall ary : arity,
-  forall val1 : Lift ary w,
-  forall val2 : Lift ary w,
-  forall e1 : Arith,
-  forall e2 : Arith,
-  evalArith ary e1 val1 ->
-  evalArith ary e2 val2 ->
-  evalArith ary (ltArith e1 e2) (apLift ary (apLift ary (returnLift ary chi_lt) val1) val2)
-| muEval :
-  forall ary : arity,
-  forall val1 : Lift (S ary) w,
-  forall val' : Lift ary w,
-  forall e1 : Arith,
-  evalArith (S ary) e1 val1 ->
-  unLiftProp ary (apLift ary (apLift ary (returnLift ary (fun f : w -> bool => fun x : w => f x = true)) (check ary val1)) val') ->
-  evalArith ary (muArith e1) (apLift ary (apLift ary (returnLift ary first_nat) (check ary val1)) val')
+Definition liftArity2 {A : Type} {B : Type} {C : Type} (n : nat) : (A -> B -> C) -> Arity n A -> Arity n B -> Arity n C :=
+  fun f : A -> B -> C => fun val1 : Arity n A => fun val2 : Arity n B => apArity n (apArity n (pureArity n f) val1) val2
 .
 
-Lemma liftEval_once :
-  forall ary : arity,
-  forall e : Arith,
-  forall val : Lift ary w,
-  evalArith ary e val ->
-  evalArith (S ary) e (returnLift 1 val).
-Proof with eauto.
-  intros ary e val H; induction H.
-  - apply (varEval (S m) n)...
-  - apply (plusEval (S ary))...
-  - apply (multEval (S ary))...
-  - apply (ltEval (S ary))...
-  - apply (muEval (S ary))... simpl...
-Qed.
-
-Lemma liftEval (n : arity) :
-  forall ary : arity,
-  forall e : Arith,
-  forall val : Lift ary w,
-  evalArith ary e val ->
-  evalArith (n + ary) e (assocLift n ary (returnLift n val)).
-Proof.
-  induction n; eauto. simpl; eauto using liftEval_once.
-Qed.
-
-Definition hasSameSemantics {A : Type} (ary : arity) (val1 : Lift ary A) (val2 : Lift ary A) : Prop :=
-  unLiftProp ary (apLift ary (apLift ary (returnLift ary (fun x : A => fun y : A => x = y)) val1) val2)
+Fixpoint assocArity (A : Type) (n : nat) : forall i : nat, Arity n (Arity i A) -> Arity (n + i) A :=
+  match n with
+  | 0 =>
+    fun i : nat =>
+    fun val : Arity i A =>
+    val
+  | S n' =>
+    fun i : nat =>
+    fun val : w -> Arity n' (Arity i A) =>
+    fun m : w =>
+    assocArity A n' i (val m)
+  end
 .
 
-Lemma hasSameSemantics_refl {A : Type} :
-  forall ary : arity,
-  forall f : Lift ary w,
-  hasSameSemantics ary f f.
+Fixpoint shiftArity_left {A : Type} (n : nat) : Arity (S n) A -> Arity n (w -> A) :=
+  match n with
+  | 0 =>
+    fun val : w -> A =>
+    val
+  | S n' =>
+    fun val : w -> Arity (S n') A =>
+    fun m : w =>
+    shiftArity_left n' (val m)
+  end
+.
+
+Fixpoint shiftArity_right {A : Type} (n : nat) : Arity n (w -> A) -> Arity (S n) A :=
+  match n with
+  | 0 =>
+    fun val : w -> A =>
+    val
+  | S n' =>
+    fun val : w -> Arity n' (w -> A) =>
+    fun m : w =>
+    shiftArity_right n' (val m)
+  end
+.
+
+Lemma pure_assoc_pure {A : Type} :
+  forall n : nat,
+  forall x : A,
+  pureArity (n + 0) x = assocArity A n 0 (pureArity n x).
 Proof with eauto.
-  unfold hasSameSemantics.
-  unfold apLift.
-  induction ary.
-  - simpl...
-  - simpl...
+  induction n... simpl. intros x. rewrite IHn...
 Qed.
 
-Lemma hasSameSemantics_symm {A : Type} :
-  forall ary : arity,
-  forall f : Lift ary A,
-  forall g : Lift ary A,
-  hasSameSemantics ary f g ->
-  hasSameSemantics ary g f.
-Proof with eauto.
-  unfold hasSameSemantics.
-  unfold apLift.
-  induction ary.
-  - simpl...
-  - simpl...
-Qed.
+Fixpoint Arity_dec (n : nat) : Arity n Prop -> Arity n Prop -> Set :=
+  match n with
+  | 0 => fun P : Prop => fun Q : Prop => {P} + {Q}
+  | S n' => fun P : w -> Arity n' Prop => fun Q : w -> Arity n' Prop => forall m : w, Arity_dec n' (P m) (Q m)
+  end
+.
 
-Lemma hasSameSemantics_trans {A : Type} :
-  forall ary : arity,
-  forall f : Lift ary A,
-  forall g : Lift ary A,
-  forall h : Lift ary A,
-  hasSameSemantics ary f g ->
-  hasSameSemantics ary g h ->
-  hasSameSemantics ary f h.
+Fixpoint Arity_ite {A : Type} (n : nat) : forall P : Arity n Prop, forall Q : Arity n Prop, Arity_dec n P Q -> Arity n A -> Arity n A -> Arity n A :=
+  match n with
+  | 0 => fun P : Prop => fun Q : Prop => fun PQ_dec : {P} + {Q} => fun val1 : A => fun val2 : A => if PQ_dec then val1 else val2
+  | S n' => fun P : w -> Arity n' Prop => fun Q : w -> Arity n' Prop => fun PQ_dec : forall m : nat, Arity_dec n' (P m) (Q m) => fun val1 : w -> Arity n' A => fun val2 : w -> Arity n' A => fun m : w => Arity_ite n' (P m) (Q m) (PQ_dec m) (val1 m) (val2 m)
+  end
+.
+
+Lemma Arity_ite_is {A : Type} :
+  forall n : nat,
+  forall R : Arity n Prop,
+  forall R_dec : Arity_dec n R (liftArity1 n (fun r : Prop => ~ r) R),
+  forall val1 : Arity n A,
+  forall val2 : Arity n A,
+  universal n (apArity n (apArity n (apArity n (apArity n (pureArity n (fun r : Prop => fun x1 : A => fun x2 : A => fun x : A => (r -> x = x1) /\ (~ r -> x = x2))) R) val1) val2) (Arity_ite n R (liftArity1 n (fun r : Prop => ~ r) R) R_dec val1 val2)).
 Proof with eauto.
-  unfold hasSameSemantics.
-  unfold apLift.
-  induction ary.
+  unfold liftArity1.
+  induction n.
   - simpl.
-    apply eq_trans.
-  - simpl...
-Qed.
-
-Lemma hasSameSemantics_liftA2 {A : Type} {B : Type} {C : Type} :
-  forall ary : arity,
-  forall f : A -> B -> C,
-  forall g1 : Lift ary A,
-  forall g2 : Lift ary A,
-  forall h1 : Lift ary B,
-  forall h2 : Lift ary B,
-  hasSameSemantics ary g1 g2 ->
-  hasSameSemantics ary h1 h2 ->
-  hasSameSemantics ary (apLift ary (apLift ary (returnLift ary f) g1) h1) (apLift ary (apLift ary (returnLift ary f) g2) h2).
-Proof with eauto.
-  unfold hasSameSemantics.
-  unfold apLift.
-  induction ary.
-  - simpl...
     intros.
-    rewrite H.
-    rewrite H0.
-    reflexivity.
+    destruct R_dec; firstorder.
   - simpl...
-Qed.
-
-Lemma eval_unique :
-  forall e : Arith,
-  forall ary : arity,
-  forall val1 : Lift ary w,
-  forall val2 : Lift ary w,
-  evalArith ary e val1 ->
-  evalArith ary e val2 ->
-  hasSameSemantics ary val1 val2.
-Proof with eauto.
-  assert ( claim1 :
-    forall ary : arity,
-    forall f1 : Lift ary (w -> bool),
-    forall f2 : Lift ary (w -> bool),
-    (forall i : Lift ary w, hasSameSemantics ary (apLift ary f1 i) (apLift ary f2 i)) ->
-    forall n1 : Lift ary w,
-    forall n2 : Lift ary w,
-    unLiftProp ary (apLift ary (apLift ary (returnLift ary (fun f : w -> bool => fun x : w => f x = true)) f1) n1) ->
-    unLiftProp ary (apLift ary (apLift ary (returnLift ary (fun f : w -> bool => fun x : w => f x = true)) f2) n2) ->
-    hasSameSemantics ary (apLift ary (apLift ary (returnLift ary first_nat) f1) n1) (apLift ary (apLift ary (returnLift ary first_nat) f2) n2)
-  ).
-  { induction ary.
-    - unfold hasSameSemantics.
-      unfold apLift.
-      simpl.
-      intros f1 f2 H.
-      assert (forall n : nat, first_nat f1 n = first_nat f2 n).
-      { induction n...
-        simpl.
-        rewrite IHn.
-        rewrite H...
-      }
-      intros.
-      rewrite H0.
-      assert (first_nat f2 n1 <= first_nat f2 n2).
-      { apply well_ordering_principle...
-        apply well_ordering_principle...
-      }
-      assert (first_nat f2 n2 <= first_nat f2 n1).
-      { apply well_ordering_principle...
-        apply well_ordering_principle...
-      }
-      lia.
-    - unfold hasSameSemantics.
-      unfold apLift.
-      simpl.
-      intros.
-      apply IHary.
-      intros.
-      apply (H (fun _ : w => i) n).
-      apply H0.
-      apply H1.
-  }
-  assert ( claim2 :
-    forall ary : arity,
-    forall n1 : Lift (S ary) w,
-    forall n2 : Lift (S ary) w,
-    hasSameSemantics (S ary) n1 n2 ->
-    forall i : Lift ary w,
-    hasSameSemantics ary (apLift ary (check ary n1) i) (apLift ary (check ary n2) i)
-  ).
-  { unfold hasSameSemantics.
-    unfold check.
-    unfold apLift.
-    induction ary.
-    - simpl...
-    - simpl.
-      intros.
-      apply IHary.
-      simpl...
-  } 
-  induction e.
-  - intros.
-    inversion H.
-    subst.
-    assert (projection a m = val1) by (apply (existsT_snd_eq (fun x : arity => Lift x w)); apply H5).
-    rewrite <- H1.
-    inversion H0.
-    subst.
-    assert (m0 = m) by lia.
-    subst m0.
-    assert (projection a m = val2) by (apply (existsT_snd_eq (fun x : arity => Lift x w)); apply H8).
-    rewrite <- H1.
-    apply (@hasSameSemantics_refl w).
-  - intros.
-    inversion H.
-    subst.
-    assert (apLift ary (apLift ary (returnLift ary plus) val0) val3 = val1) by (apply (existsT_snd_eq (fun x : arity => Lift x w)); apply H4).
-    inversion H0.
-    subst.
-    assert (apLift ary (apLift ary (returnLift ary plus) val4) val5 = val2) by (apply (existsT_snd_eq (fun x : arity => Lift x w)); apply H8).
-    subst.
-    apply hasSameSemantics_liftA2...
-  - intros.
-    inversion H.
-    subst.
-    assert (apLift ary (apLift ary (returnLift ary mult) val0) val3 = val1) by (apply (existsT_snd_eq (fun x : arity => Lift x w)); apply H4).
-    inversion H0.
-    subst.
-    assert (apLift ary (apLift ary (returnLift ary mult) val4) val5 = val2) by (apply (existsT_snd_eq (fun x : arity => Lift x w)); apply H8).
-    subst.
-    apply hasSameSemantics_liftA2...
-  - intros.
-    inversion H.
-    subst.
-    assert (apLift ary (apLift ary (returnLift ary chi_lt) val0) val3 = val1) by (apply (existsT_snd_eq (fun x : arity => Lift x w)); apply H4).
-    inversion H0.
-    subst.
-    assert (apLift ary (apLift ary (returnLift ary chi_lt) val4) val5 = val2) by (apply (existsT_snd_eq (fun x : arity => Lift x w)); apply H8).
-    subst.
-    apply hasSameSemantics_liftA2...
-  - intros.
-    inversion H.
-    inversion H0.
-    subst.
-    assert ((apLift ary (apLift ary (returnLift ary first_nat) (check ary val0)) val') = val1) by (apply (existsT_snd_eq (fun x : arity => Lift x w)); apply H2).
-    assert ((apLift ary (apLift ary (returnLift ary first_nat) (check ary val3)) val'0) = val2) by (apply (existsT_snd_eq (fun x : arity => Lift x w)); apply H7).
-    subst.
-    apply claim1...
-Qed.
-
-Definition correspondsToFunc (ary : arity) (func1 : Lift ary w) (func : Lift ary w) : Prop :=
-  unLiftProp ary (apLift ary (apLift ary (returnLift ary (fun x : w => fun y : w => x = y)) func) func1)
-.
-
-Example correspondsToFunc_ex1 (f : Lift 2 w) :
-  correspondsToFunc 2 (fun x1 : w => fun x0 : w => f x1 x0) (apLift 2 (apLift 2 (returnLift 2 f) (projection 1 0)) (projection 0 1)).
-Proof.
-  unfold correspondsToFunc.
-  unfold apLift.
-  simpl.
-  reflexivity.
-Qed.
-
-Definition correspondsToRel (ary : arity) (func1 : Lift ary w) (rel : Lift ary Prop) : Prop :=
-  unLiftProp ary (apLift ary (apLift ary (returnLift ary (fun p : Prop => fun x : w => (~ ~ p -> x = 0) /\ (~ p -> x = 1))) rel) func1)
-.
-
-Example correspondsToRel_ex1 :
-  correspondsToRel 2 (fun x1 : w => fun x0 : w => chi_lt x1 x0) (apLift 2 (apLift 2 (returnLift 2 lt) (projection 1 0)) (projection 0 1)).
-Proof.
-  unfold correspondsToRel.
-  unfold chi_lt.
-  unfold projection.
-  unfold apLift.
-  simpl.
-  intros n1 n2.
-  destruct (Compare_dec.lt_dec n1 n2); lia.
-Qed.
-
-Inductive IsRecursivelyEnumerable : forall ary : arity, Lift ary Prop -> Prop :=
-| IsRE :
-  forall e : Arith,
-  forall ary : arity,
-  forall func1 : Lift (S ary) w,
-  forall rel1 : Lift (S ary) Prop,
-  forall rel : Lift ary Prop,
-  evalArith (S ary) e func1 ->
-  correspondsToRel (S ary) func1 rel1 ->
-  unLiftProp ary (apLift ary (apLift ary (returnLift ary (fun P : Prop => fun Q : w -> Prop => P <-> exists x : w, Q x)) rel) (shiftLift_left ary rel1)) -> 
-  IsRecursivelyEnumerable ary rel
-.
-
-Fixpoint numEval (n : nat) : Lift 0 w :=
-  match n with
-  | 0 => apLift 0 (apLift 0 (returnLift 0 first_nat) (check 0 (fun x : w => x))) 0
-  | S n' => apLift 0 (apLift 0 (returnLift 0 first_nat)) (check 0 (shiftLift_left 0 (fun x : w => chi_lt (numEval n') x))) (S (numEval n'))
-  end
-.
-
-Lemma numEval_correpondsTo_numeral :
-  forall n : nat,
-  correspondsToFunc 0 (numEval n) n.
-Proof with eauto.
-  assert ( claim1 :
-    forall n : nat,
-    S n = first_nat (fun x : w => (if Compare_dec.lt_dec n x then 0 else 1) =? 0) (S n)
-  ).
-  { assert (forall n : nat, forall p : nat -> bool, first_nat p n <= n).
-    { induction n...
-      simpl.
-      intros p.
-      destruct (p (first_nat p n)) eqn: H0...
-    }
-    intros n.
-    assert (first_nat (fun x : w => (if Compare_dec.lt_dec n x then 0 else 1) =? 0) (S n) <= S n) by apply H.
-    set (p := (fun x : w => (if Compare_dec.lt_dec n x then 0 else 1) =? 0)).
-    assert (p (first_nat p (S n)) = true).
-    { apply well_ordering_principle...
-      unfold p.
-      destruct (Compare_dec.lt_dec n (S n))...
-    }
-    unfold p in H1.
-    destruct (Compare_dec.lt_dec n (first_nat (fun x : w => (if Compare_dec.lt_dec n x then 0 else 1) =? 0) (S n))).
-    - unfold p.
-      lia.
-    - inversion H1.
-  }
-  induction n.
-  - reflexivity.
-  - unfold correspondsToFunc in *.
-    unfold check in *.
-    unfold apLift in *.
-    unfold chi_lt in *.
-    simpl in *.
-    rewrite <- IHn...
-Qed.
-
-Fixpoint numArith (n : nat) : Arith :=
-  match n with
-  | 0 => muArith (varArith 0)
-  | S n' => muArith (ltArith (numArith n') (varArith 0))
-  end
-.
-
-Lemma eval_numArith_numEval :
-  forall n : nat,
-  evalArith 0 (numArith n) (numEval n).
-Proof with eauto.
-  induction n.
-  - apply muEval.
-    + apply (varEval 0 0).
-    + reflexivity.
-  - simpl.
-    assert (n = numEval n) by apply numEval_correpondsTo_numeral.
-    cut (evalArith 0 (muArith (ltArith (numArith n) (varArith 0))) (apLift 0 (apLift 0 (returnLift 0 first_nat)) (check 0 (shiftLift_left 0 (fun x : w => chi_lt n x))) (S n))).
-    { unfold apLift.
-      simpl.
-      rewrite <- H...
-    }
-    apply (muEval 0 (fun x : w => chi_lt n x) (S n)).
-    + apply (ltEval 1).
-      * apply liftEval_once...
-        rewrite <- H in IHn...
-      * apply (varEval 0 0).
-    + unfold apLift.
-      simpl.
-      unfold check.
-      simpl.
-      unfold apLift.
-      simpl.
-      unfold chi_lt.
-      destruct (Compare_dec.lt_dec n (S n))...
-Qed.
-
-Definition notEval (ary : arity) (func1 : Lift ary w) : Lift ary w :=
-  apLift ary (apLift ary (returnLift ary chi_lt) (returnLift ary 0)) func1
-.
-
-Lemma notEval_correpondsTo_negation :
-  forall ary : arity,
-  forall P1 : Lift ary Prop,
-  forall func1 : Lift ary w,
-  correspondsToRel ary func1 P1 ->
-  correspondsToRel ary (notEval ary func1) (apLift ary (returnLift ary (fun p1 : Prop => ~ p1)) P1).
-Proof with eauto.
-  assert ( claim1 :
-    forall ary : arity,
-    forall P : Lift ary Prop,
-    forall func1 : Lift ary w,
-    unLiftProp ary (bindLift ary (bindLift ary (returnLift ary (fun (p : Prop) (x : w) => (~ ~ p -> x = 0) /\ (~ p -> x = 1))) (fun f' : Prop -> w -> Prop => bindLift ary P (fun x' : Prop => returnLift ary (f' x')))) (fun f' : w -> Prop => bindLift ary func1 (fun x' : w => returnLift ary (f' x')))) ->
-    unLiftProp ary (apLift ary (apLift ary (returnLift ary (fun (p : Prop) (x : w) => (~ ~ p -> x = 0) /\ (~ p -> x = 1))) (bindLift ary (returnLift ary (fun p : Prop => ~ p)) (fun f' : Prop -> Prop => bindLift ary P (fun x' : Prop => returnLift ary (f' x'))))) (apLift ary (apLift ary (returnLift ary chi_lt) (returnLift ary 0)) func1))
-  ).
-  { induction ary.
-    - unfold apLift.
-      simpl.
-      intros.
-      unfold chi_lt.
-      destruct (Compare_dec.lt_dec 0 func1 ).
-      * constructor...
-        intros.
-        assert (func1 = 0) by tauto.
-        lia.
-      * assert (func1 = 0) by lia.
-        constructor...
-        intros.
-        assert (func1 = 1) by tauto.
-        lia.
-    - unfold apLift.
-      simpl...
-  }
-  unfold correspondsToRel...
-Qed.
-
-Definition notArith (e1 : Arith) : Arith :=
-  ltArith (numArith 0) e1
-.
-
-Lemma eval_notArith_notEval :
-  forall e1 : Arith,
-  forall ary : arity,
-  forall func1 : Lift ary w,
-  evalArith ary e1 func1 ->
-  evalArith ary (notArith e1) (notEval ary func1).
-Proof with eauto.
-  unfold notEval.
-  unfold notArith.
-  intros.
-  apply ltEval...
-  assert (ary = ary + 0)...
-  rewrite H0.
-  rewrite (assoc_return ary).
-  apply liftEval.
-  apply eval_numArith_numEval.
-Qed.
-
-Definition orEval (ary : arity) (func1 : Lift ary w) (func2 : Lift ary w) : Lift ary w :=
-  apLift ary (apLift ary (returnLift ary mult) func1) func2
-.
-
-Lemma orEval_correspondsTo_disjunction :
-  forall ary : arity,
-  forall P1 : Lift ary Prop,
-  forall P2 : Lift ary Prop,
-  forall func1 : Lift ary w,
-  forall func2 : Lift ary w,
-  correspondsToRel ary func1 P1 ->
-  correspondsToRel ary func2 P2 ->
-  correspondsToRel ary (orEval ary func1 func2) (apLift ary (apLift ary (returnLift ary (fun p1 : Prop => fun p2 : Prop => p1 \/ p2)) P1) P2).
-Proof with eauto. 
-  assert ( claim1 :
-    forall ary : arity,
-    forall P1 : Lift ary Prop,
-    forall P2 : Lift ary Prop,
-    forall func1 : Lift ary w,
-    forall func2 : Lift ary w,
-    unLiftProp ary (bindLift ary (bindLift ary (returnLift ary (fun (p : Prop) (x : w) => (~ ~ p -> x = 0) /\ (~ p -> x = 1))) (fun f' : Prop -> w -> Prop => bindLift ary P1 (fun x' : Prop => returnLift ary (f' x')))) (fun f' : w -> Prop => bindLift ary func1 (fun x' : w => returnLift ary (f' x')))) ->
-    unLiftProp ary (bindLift ary (bindLift ary (returnLift ary (fun (p : Prop) (x : w) => (~ ~ p -> x = 0) /\ (~ p -> x = 1))) (fun f' : Prop -> w -> Prop => bindLift ary P2 (fun x' : Prop => returnLift ary (f' x')))) (fun f' : w -> Prop => bindLift ary func2 (fun x' : w => returnLift ary (f' x')))) ->
-    unLiftProp ary (apLift ary (apLift ary (returnLift ary (fun (p : Prop) (x : w) => (~ ~ p -> x = 0) /\ (~ p -> x = 1))) (bindLift ary (bindLift ary (returnLift ary (fun p1 p2 : Prop => p1 \/ p2)) (fun f' : Prop -> Prop -> Prop => bindLift ary P1 (fun x' : Prop => returnLift ary (f' x')))) (fun f' : Prop -> Prop => bindLift ary P2 (fun x' : Prop => returnLift ary (f' x'))))) (apLift ary (apLift ary (returnLift ary Init.Nat.mul) func1) func2))
-  ).
-  { induction ary.
-    - unfold apLift.
-      simpl.
-      intros.
-      constructor.
-      + intros.
-        assert (~ (func1 <> 0 /\ func2 <> 0)) by tauto.
-        lia.
-      + intros.
-        assert (func1 = 1) by tauto.
-        assert (func2 = 1) by tauto.
-        lia.
-    - unfold apLift.
-      simpl...
-  }
-  unfold orEval.
-  unfold correspondsToRel...
-Qed.
-
-Definition orArith (e1 : Arith) (e2 : Arith) : Arith :=
-  multArith e1 e2
-.
-
-Lemma eval_orArith_orEval :
-  forall e1 : Arith,
-  forall e2 : Arith,
-  forall ary : arity,
-  forall func1 : Lift ary w,
-  forall func2 : Lift ary w,
-  evalArith ary e1 func1 ->
-  evalArith ary e2 func2 ->
-  evalArith ary (orArith e1 e2) (orEval ary func1 func2).
-Proof with eauto.
-  intros.
-  unfold orArith.
-  unfold orEval.
-  apply multEval...
-Qed.
-
-Definition andEval (ary : arity) (func1 : Lift ary w) (func2 : Lift ary w) : Lift ary w :=
-  notEval ary (orEval ary (notEval ary func1) (notEval ary func2))
-.
-
-Lemma andEval_correpondsTo_conjunction :
-  forall ary : arity,
-  forall P1 : Lift ary Prop,
-  forall P2 : Lift ary Prop,
-  forall func1 : Lift ary w,
-  forall func2 : Lift ary w,
-  correspondsToRel ary func1 P1 ->
-  correspondsToRel ary func2 P2 ->
-  correspondsToRel ary (andEval ary func1 func2) (apLift ary (apLift ary (returnLift ary (fun p1 : Prop => fun p2 : Prop => p1 /\ p2)) P1) P2).
-Proof with eauto.
-  unfold correspondsToRel.
-  unfold andEval.
-  intros.
-  unfold apLift in H.
-  unfold apLift in H0.
-  generalize dependent ary.
-  induction ary.
-  - intros.
-    assert (correspondsToRel 0 (notEval 0 (orEval 0 (notEval 0 func1) (notEval 0 func2))) (apLift 0 (apLift 0 (returnLift 0 (fun p1 p2 : Prop => ~ (~ p1 \/ ~ p2))) P1) P2)).
-    { apply (notEval_correpondsTo_negation 0).
-      apply (orEval_correspondsTo_disjunction 0).
-      - apply (notEval_correpondsTo_negation 0)...
-      - apply (notEval_correpondsTo_negation 0)...
-    }
-    unfold correspondsToRel in H1.
-    unfold correspondsToRel.
-    unfold apLift in *.
-    simpl in *.
-    tauto.
-  - unfold orEval.
-    unfold notEval.
-    unfold apLift.
-    simpl...
-Qed.
-
-Definition andArith (e1 : Arith) (e2 : Arith) : Arith :=
-  notArith (orArith (notArith e1) (notArith e2))
-.
-
-Lemma eval_andArith_andEval :
-  forall e1 : Arith,
-  forall e2 : Arith,
-  forall ary : arity,
-  forall func1 : Lift ary w,
-  forall func2 : Lift ary w,
-  evalArith ary e1 func1 ->
-  evalArith ary e2 func2 ->
-  evalArith ary (andArith e1 e2) (andEval ary func1 func2).
-Proof with eauto.
-  intros.
-  apply eval_notArith_notEval.
-  apply eval_orArith_orEval.
-  apply eval_notArith_notEval...
-  apply eval_notArith_notEval...
-Qed.
-
-Definition eqEval (ary : arity) (func1 : Lift ary w) (func2 : Lift ary w) : Lift ary w :=
-  andEval ary (notEval ary (apLift ary (apLift ary (returnLift ary chi_lt) func1) func2)) (notEval ary ((apLift ary (apLift ary (returnLift ary chi_lt) func2) func1)))
-.
-
-Lemma eqEval_correspondsTo_equality :
-  forall ary : arity,
-  forall val1 : Lift ary w,
-  forall val2 : Lift ary w,
-  forall func1 : Lift ary w,
-  forall func2 : Lift ary w,
-  correspondsToFunc ary func1 val1 ->
-  correspondsToFunc ary func2 val2 ->
-  correspondsToRel ary (eqEval ary func1 func2) (apLift ary (apLift ary (returnLift ary (fun x : w => fun y : w => x = y)) val1) val2).
-Proof with eauto.
-  unfold correspondsToFunc.
-  unfold correspondsToRel.
-  unfold eqEval.
-  intros.
-  unfold apLift in H.
-  unfold apLift in H0.
-  generalize dependent ary.
-  induction ary.
-  - intros.
-    simpl.
-    assert (correspondsToRel 0 (eqEval 0 func1 func2) (apLift 0 (apLift 0 (returnLift 0 (fun x1 : w => fun x2 : w => (~ (x1 < x2) /\ ~ (x2 < x1)))) val1) val2)).
-    { unfold eqEval.
-      apply (andEval_correpondsTo_conjunction 0).
-      - apply (notEval_correpondsTo_negation 0)...
-        unfold apLift.
-        simpl.
-        unfold chi_lt.
-        unfold correspondsToFunc in *.
-        unfold correspondsToRel.
-        unfold apLift in *.
-        simpl in *.
-        destruct (Compare_dec.lt_dec func1 func2); lia.
-      - apply (notEval_correpondsTo_negation 0)...
-        unfold apLift.
-        simpl.
-        unfold chi_lt.
-        unfold correspondsToFunc in *.
-        unfold correspondsToRel.
-        unfold apLift in *.
-        simpl in *.
-        destruct (Compare_dec.lt_dec func2 func1); lia.
-    }
-    unfold correspondsToRel in H1.
-    unfold apLift in *.
-    simpl in *...
-    destruct H1.
-    constructor.
-    + intros.
-      apply H1.
-      lia.
-    + intros.
-      apply H2.
-      lia.
-  - unfold andEval.
-    unfold notEval.
-    unfold orEval.
-    unfold apLift.
-    simpl...
-Qed.
-
-Definition eqArith (e1 : Arith) (e2 : Arith) : Arith :=
-  andArith (notArith (ltArith e1 e2)) (notArith (ltArith e2 e1))
-.
-
-Lemma eval_eqArith_eqEval :
-  forall e1 : Arith,
-  forall e2 : Arith,
-  forall ary : arity,
-  forall func1 : Lift ary w,
-  forall func2 : Lift ary w,
-  evalArith ary e1 func1 ->
-  evalArith ary e2 func2 ->
-  evalArith ary (eqArith e1 e2) (eqEval ary func1 func2).
-Proof with eauto.
-  intros.
-  apply eval_andArith_andEval.
-  - apply eval_notArith_notEval.
-    apply ltEval...
-  - apply eval_notArith_notEval.
-    apply ltEval...
 Qed.
 
 End Arithmetic.
